@prefix rdf: <http://www.w3.org/1999/02/22-rdf-syntax-ns#> .
@prefix rdfs: <http://www.w3.org/2000/01/rdf-schema#> .
@prefix owl:  <http://www.w3.org/2002/07/owl#> .
@prefix prov: <http://www.w3.org/ns/prov#> .
@prefix obo:  <http://purl.obolibrary.org/obo/> .
@base <https://raw.githubusercontent.com/BFO-Mappings/BFO-Mappings/main/PROV/prov-bfo-directmappings.ttl> .

<https://raw.githubusercontent.com/BFO-Mappings/BFO-Mappings/main/PROV/prov-bfo-directmappings.ttl>
   a                     owl:Ontology;
   rdfs:label           "Basic Formal Ontology (BFO) mappings for W3C PROVenance Interchange Ontology (PROV-O)"@en ;
   owl:versionInfo      "2023-09-29"@en ;
   owl:versionIRI       <http://www.w3.org/ns/prov-bfo-directmappings-20230718> ;
   rdfs:seeAlso         <http://www.w3.org/ns/prov> ,
                        <https://basic-formal-ontology.org/> ,
                        <https://github.com/BFO-Mappings/BFO-Mappings> ,
                        <https://github.com/bfo-ontology/bfo-2020> ;
.

# Class mappings
prov:Entity               rdfs:comment "A prov:Entity is a continuant because it entirely exists at different times. However, a prov:Entity is not a spatial region because spatial regions are causally inert and may not particpate in processes."@en ;
                          rdfs:equivalentClass [ rdf:type owl:Class ;
                                            owl:unionOf ( obo:BFO_0000020 # specifically dependent continuant
                                                          obo:BFO_0000031 # generically dependent continuant
                                                          [ owl:intersectionOf ( obo:BFO_0000004 # independent continuant
                                                                                [ rdf:type owl:Class ;
                                                                                  owl:complementOf obo:BFO_0000006 # spatial region
                                                                                ]
                                                                              ) ;
                                                            rdf:type owl:Class
                                                          ]
                                                        )
                                          ] .


prov:Agent                rdfs:comment "A prov:Agent is a material entity because always has some matter as a part that persists in time. A prov:Agent participates in some prov:Activity at some time and bears a role, that, if realized, is realized in a prov:Activity taking place. According to Requirement VI13 in 'Rationale of Prov', this could be a prov:Entity."@en ;
                          rdfs:subClassOf [ owl:intersectionOf ( obo:BFO_0000040 # material entity
                                                                  [ rdf:type owl:Restriction ;
                                                                    owl:onProperty obo:BFO_0000056 ; # participates in at some time
                                                                    owl:someValuesFrom prov:Activity
                                                                  ]
                                                                  [ rdf:type owl:Restriction ;
                                                                    owl:onProperty obo:BFO_0000196 ; # bearer of
                                                                    owl:someValuesFrom [ owl:intersectionOf ( obo:BFO_0000023 # role
                                                                                                              [ rdf:type owl:Restriction ;
                                                                                                                owl:onProperty obo:BFO_0000054 ; # realized in / has realization
                                                                                                                owl:someValuesFrom prov:Activity
                                                                                                              ]
                                                                                                            ) ;
                                                                                        rdf:type owl:Class
                                                                                      ]
                                                                  ]
                                                                ) ;
                                            rdf:type owl:Class
                                          ] .


obo:BFO_0000015           rdfs:comment "A prov:Activity is equivalent to a process because it occurs over time, while not being a temporal region itself."@en ;
                          owl:equivalentClass prov:Activity .


prov:Location             rdfs:comment "A prov:location is equivalent to a site because a prov:Location is a three-dimensional immaterial entity that is (partially or wholly) bounded by a material entity or it is a three-dimensional immaterial part), but adds specificity in that it can be an ISO 19112 geographic place or another location in which provenance occurs."@en ;
                          owl:equivalentClass obo:BFO_0000029 . # site


prov:InstantaneousEvent   rdfs:comment "An prov:InstantaneousEvent is equivalent to a process boundary because it is referred to as the boundary (start or end) of a prov:Activity as an occurrent."@en ;
                          owl:equivalentClass obo:BFO_0000035 . # process boundary


prov:Plan                 rdfs:comment "A prov:Plan exists in virtue of the fact that there is at least one of what may be multiple copies; it is the content or the pattern that the multiple copies share."@en ;
                          rdfs:subClassOf obo:BFO_0000031 . # generically dependent continuant


prov:Role                 rdfs:comment "A prov:Role is a bfo:role because its externally determined by the context in which the bearer plays the role."@en ;
                          rdfs:subClassOf obo:BFO_0000023 . # role TODO: realized in an Activity? need to resolve issue with prov:hadRole


prov:Influence            rdfs:comment "A prov:Influence is either a process or process boundary, but not both at once, because it occurs over time or at an instant in time. Although prov:Influence is defined as a capacity, all of its subclasses are clearly defined as occurring over time or at an instant."@en ;
                          owl:disjointUnionOf ( obo:BFO_0000015  # process, e.g. prov:Derivation
                                                obo:BFO_0000035  # process boundary, e.g. prov:Generation is a prov:InstantaneousEvent
                                            ) .


prov:Dictionary           rdfs:comment "A prov:Dictionary exists in virtue of the fact that there is at least one of what may be multiple copies; it is the content or the pattern that the multiple copies share."@en ;
                          rdfs:subClassOf obo:BFO_0000031 . # generically dependent continuant


prov:KeyEntityPair        rdfs:comment "A prov:KeyEntityPair exists in virtue of the fact that there is at least one of what may be multiple copies; it is the content or the pattern that the multiple copies share."@en ;
                          rdfs:subClassOf obo:BFO_0000031 . # generically dependent continuant


# TODO: commentary on why prov:ServiceDescription isn't an Agent


# Object Properties
prov:hadMember            rdfs:comment "A prov:Collection that has member some prov:Entity also has it as a part."@en ;
                          rdfs:subPropertyOf obo:BFO_00000178 . # has continuant part (at some time)

prov:hadGeneration        rdfs:comment "A prov:Derivation that has generation some prov:Generation also has it as a temporal part."@en ;
                          rdfs:subPropertyOf obo:BFO_0000121 . # has temporal part

prov:hadActivity          rdfs:comment "A prov Delegation or Derivation or End or Start that has activity some prov:Activity is also a temporal part of that prov:Activity."@en ;
                          rdfs:subPropertyOf obo:BFO_0000139 . # temporal part of

prov:qualifiedStart       rdfs:comment "A prov:Activity whose qualified start is some prov:Start has it as a temporal part."@en ;
                          rdfs:subPropertyOf obo:BFO_0000121 . # has temporal part
                          
prov:qualifiedEnd         rdfs:comment "A prov:Activity whose qualified end is some prov:End has it as a temporal part."@en ;
                          rdfs:subPropertyOf obo:BFO_0000121 . # has temporal part

prov:qualifiedUsage       rdfs:comment "A prov:Activity whose qualified usage is some prov:Usage has it as a temporal part."@en ;
                          rdfs:subPropertyOf obo:BFO_0000121 . # has temporal part

prov:hadUsage             rdfs:comment "A prov:Derivation that had usage some prov:Usage has it as a temporal part."@en ;
                          rdfs:subPropertyOf obo:BFO_0000121 . # has temporal part

prov:hadDictionaryMember  rdfs:comment "A prov:Dictionary has a prov:Key-Entity Pair as a member, then it has it as a continuant part at some time."@en ;
                          rdfs:subPropertyOf obo:BFO_00000178 . # has continuant part (at some time)

# prov:atLocation           rdfs:subPropertyOf obo:BFO_0000066 ; # has to be disjoint union of "occurs in" or "located in"
#                           rdfs:comment "If a prov Activity, Agent, or Entity is at some Location, then it occurs in or is located in that Location"@en .
