@prefix rdf: <http://www.w3.org/1999/02/22-rdf-syntax-ns#> .
@prefix rdfs: <http://www.w3.org/2000/01/rdf-schema#> .
@prefix owl:  <http://www.w3.org/2002/07/owl#> .
@prefix prov: <http://www.w3.org/ns/prov#> .
@prefix obo:  <http://purl.obolibrary.org/obo/> .
@base <https://raw.githubusercontent.com/BFO-Mappings/BFO-Mappings/main/PROV/prov-bfo-directmappings.ttl> .

<https://raw.githubusercontent.com/BFO-Mappings/BFO-Mappings/main/PROV/prov-bfo-directmappings.ttl>
   a                     owl:Ontology;
   rdfs:label           "Basic Formal Ontology (BFO) mappings for W3C PROVenance Interchange Ontology (PROV-O)"@en ;
   owl:versionInfo      "2023-07-18"@en ;
   owl:versionIRI       <http://www.w3.org/ns/prov-bfo-directmappings-20230718> ;
   rdfs:seeAlso         <http://www.w3.org/ns/prov> ,
                        <https://basic-formal-ontology.org/> ,
                        <https://github.com/bfo-ontology/bfo-2020> ;
.

# Class mappings
# Entities are continuants, except for spatial regions (which are causally inert and may not participate in processes)
prov:Entity               rdfs:subClassOf [ rdf:type owl:Class ;
                                            owl:unionOf ( obo:BFO_0000020  # specifically dependent continuant
                                                          obo:BFO_0000031  # generically dependent continuant
                                                          [ owl:intersectionOf ( obo:BFO_0000004  # independent continuant
                                                                                [ rdf:type owl:Class ;
                                                                                  owl:complementOf obo:BFO_0000006  # spatial region
                                                                                ]
                                                                               ) ;
                                                            rdf:type owl:Class ;
                                                          ]
                                                        )
                                          ] .
                          rdfs:comment "A prov:entity is a continuant because it entirely exists at different times. However, a prov:Entity is not a spatial region because spatial regions are causally inert and may not particpate in processes."@en .

                          
prov:Agent                owl:disjointUnionOf (
                                                [ owl:intersectionOf ( obo:BFO_0000040 # material entity (could be a prov:Entity per Requirement VI13 in "Rationale of Prov")
                                                                        [ rdf:type owl:Restriction ; # anonymous 'agent role'
                                                                          owl:onProperty obo:BFO_0000196 ; # bearer of
                                                                          owl:someValuesFrom [ owl:intersectionOf ( obo:BFO_0000023 # role
                                                                                                                    [ rdf:type owl:Restriction ;
                                                                                                                      owl:onProperty obo:BFO_0000054 ; # has realization
                                                                                                                      owl:someValuesFrom prov:Activity
                                                                                                                    ]
                                                                                                                  ) ;
                                                                                              rdf:type owl:Class
                                                                                            ]
                                                                        ]
                                                                      ) ;
                                                  rdf:type owl:Class
                                                ]
                                                prov:Activity # process (could be a prov:Activity as per Requirement VI4 in "Rationale of Prov")
                                              ) ;
                          rdfs:comment  "An agent is a material entity because it always has some matter as a part that persists in time"@en .
                          rdfs:comment  "An agent, if it's a material entity, bears a role, that, if realized, is realized in an activity taking place"@en .


prov:Activity             rdfs:subClassOf obo:BFO_0000015 ; # process
                          rdfs:comment "An activity is a process because it happens over time, while not being a temporal region itself"@en .


prov:Role                 rdfs:subClassOf obo:BFO_0000023 ; # role
                          rdfs:comment "A prov:role is a bfo:role because its externally determined by the context in which the bearer plays the role"@en .


prov:Location             rdfs:subClassOf obo:BFO_0000029 ; # site
                          rdfs:comment "A location is a subclass of site as the prov:Location term fits under the BFO:site defiition (a three-dimensional immaterial entity that is (partially or wholly) bounded by a material entity or it is a three-dimensional immaterial part) but adds specificity in that it can be an ISO 19112 geographic place or another location in which provenance occurs "@en .


prov:InstantaneousEvent   rdfs:subClassOf obo:BFO_0000035 ; # process boundary
                          rdfs:comment "An instantaneous event is a process boundary because it is referred to as the boundary (start or end) of an activity as an occurrent"@en .


prov:Plan                 rdfs:subClassOf obo:BFO_0000031 ; # generically dependent continuant
                          rdfs:comment "Plans exists in virtue of the fact that there is at least one of what may be multiple copies; it is the content or the pattern that the multiple copies share"@en .


prov:Influence            owl:disjointUnionOf ( obo:BFO_0000015  # process, e.g. prov:Derivation
                                                obo:BFO_0000035  # process boundary, e.g. prov:Generation is a prov:InstantaneousEvent
                                             ) ;
                          rdfs:comment "Influences are either processes or process boundaries, but not both at once, because they occur over time or at an instant in time. Although influence is defined as a capacity, all of its subclasses are clearly defined as occurring over time or at an instant."@en .


# Object Properties
prov:hadMember            rdfs:subPropertyOf obo:BFO_0000051 . # has part
prov:hadGeneration        rdfs:subPropertyOf obo:BFO_0000121 . # has temporal part
prov:hadActivity          rdfs:subPropertyOf obo:BFO_0000139 . # temporal part of
prov:qualifiedStart       rdfs:subPropertyOf obo:BFO_0000121 . # has temporal part
prov:qualifiedEnd         rdfs:subPropertyOf obo:BFO_0000121 . # has temporal part
prov:qualifiedUsage       rdfs:subPropertyOf obo:BFO_0000121 . # has temporal part