@prefix rdf: <http://www.w3.org/1999/02/22-rdf-syntax-ns#> .
@prefix rdfs: <http://www.w3.org/2000/01/rdf-schema#> .
@prefix owl:  <http://www.w3.org/2002/07/owl#> .
@prefix prov: <http://www.w3.org/ns/prov#> .
@prefix obo:  <http://purl.obolibrary.org/obo/> .
@base <https://raw.githubusercontent.com/BFO-Mappings/BFO-Mappings/main/PROV/prov-ro-directmappings.ttl> .

<https://raw.githubusercontent.com/BFO-Mappings/BFO-Mappings/main/PROV/prov-ro-directmappings.ttl>
   a                     owl:Ontology;
   rdfs:label           "Relation Ontology (RO) mappings for W3C PROVenance Interchange Ontology (PROV-O)"@en ;
   owl:versionInfo      "2023-07-19"@en ;
   owl:versionIRI       <http://www.w3.org/ns/prov-ro-directmappings-20230718> ;
   owl:imports          <https://raw.githubusercontent.com/BFO-Mappings/BFO-Mappings/main/PROV/prov-bfo-directmappings.ttl> ;
   rdfs:seeAlso         <http://www.w3.org/ns/prov> ,
                        <https://obofoundry.org/ontology/ro.html> ;
.

# Object Property mappings
prov:influenced           rdfs:subPropertyOf obo:RO_0002410 ; #causally related to
                          rdfs:comment "An entity may influence another entity and this is a causal relation."@en .
prov:wasAttributedTo      rdfs:subPropertyOf obo:RO_0002559 ; #causally influenced by
                          rdfs:comment "An entity may be attributed to an agent, and this is a causal influence by the agent"@en .
prov:alternateOf          rdfs:subPropertyOf obo:RO_0002559 ; #causally influenced by
                          rdfs:comment "An entity may be an alternate of an entity, and this is a causal relation."@en .
prov:wasDerivedFrom       rdfs:subPropertyOf obo:RO_0002559 ; #causally influenced by
                          rdfs:comment "An entity may be derived from an entity, being causally influenced by it."@en .

prov:wasEndedBy           rdfs:subPropertyOf obo:RO_0000057 ; #has participant
                          rdfs:comment "A process has a (non spatial region) continuant as a participant. An activity is a process that may be ended by a prov:entity as a participant."@en .
prov:wasStartedBy         rdfs:subPropertyOf obo:RO_0000057 ; #has participant
                          rdfs:comment "A process has a (non spatial region) continuant as a participant. An activity is a process that may be started by a prov:entity as a participant."@en .
prov:wasAssociatedWith    rdfs:subPropertyOf obo:RO_0000057 ; #has participant
                          rdfs:comment "A process has a (non spatial region) continuant as a participant. An activity is a process that may be associated with a prov:entity as a participant."@en .
prov:invalidated          rdfs:subPropertyOf obo:RO_0000057 ; #has participant
                          rdfs:comment "A process has a (non spatial region) continuant as a participant. An activity is a process that may be invalidated by a prov:entity as a participant."@en .
prov:used                 rdfs:subPropertyOf obo:RO_0000057 ; #has participant
                          rdfs:comment "A process has a (non spatial region) continuant as a participant. An activity is a process that may use a prov:entity as a participant."@en .
prov:generated            rdfs:subPropertyOf obo:RO_0000057 ; #has participant
                          rdfs:comment "An activity is a process that may be generated by a prov:entity as a participant."@en .

prov:wasInvalidatedBy     rdfs:subPropertyOf obo:RO_0000056 ; #participates in
                          rdfs:comment "An entity (non-spatial region continuant) may participate in its invalidation by an activity (process)"@en .
prov:wasGeneratedBy       rdfs:subPropertyOf obo:RO_0000056 ; #participates in
                          rdfs:comment "An entity (non-spatial region continuant) may participate in its generation by an activity (process)"@en .

prov:wasInformedBy            rdfs:subPropertyOf obo:RO_0002501 ; #causal relation between processes
                              rdfs:comment "An activity may inform an activity. Both are processes and this is a causal relation."@en .
prov:hadGeneration            rdfs:subPropertyOf obo:RO_0002501 ; #causal relation between processes
                              rdfs:comment "An activity may generate another activity. Both are processes and this is a causal relation."@en .
prov:hadUsage                 rdfs:subPropertyOf obo:RO_0002501 ; #causal relation between processes
                              rdfs:comment "A derivation may use a usage. Both are processes and this is a causal relation."@en .

prov:qualifiedAssociation     rdfs:subPropertyOf obo:RO_0002501 ; #causal relation between processes
                              rdfs:comment "An activity may be associated with an activity. Both are processes and this is a causal relation."@en .
prov:qualifiedCommunication   rdfs:subPropertyOf obo:RO_0002501 ; #causal relation between processes
                              rdfs:comment "An activity may communicate another activity. Both are processes and this is a causal relation. For example: A wasInfomedBy B = A and B are both prov:activities, and A was causally related to B such that A utilizes a provenance_entity that wasGeneratedBy B"@en .
prov:qualifiedStart           rdfs:subPropertyOf obo:RO_0002501 ; #causal relation between processes
                              rdfs:comment "An activity may start an activity. Both are processes and this is a causal relation."@en .

prov:hadMember                rdfs:subPropertyOf obo:RO_0002351 ; #has member
                              rdfs:comment "Establish a relationship between similar BFO/RO and PROV terms - PROV term is more specific than the RO has member relation, and hence is a subclass of the RO term "@en .

# Other property restrictions
prov:Agent rdf:type owl:Class ;
           rdfs:subClassOf [ rdf:type owl:Class ;
                             owl:unionOf ( prov:Activity
                                           [ owl:intersectionOf ( obo:BFO_0000040 # material entity
                                                                  [ rdf:type owl:Restriction ; # anonymous 'agent role'
                                                                    owl:onProperty obo:RO_0000087 ; # has role
                                                                    owl:someValuesFrom [ owl:intersectionOf ( obo:BFO_0000023 # role
                                                                                                              [ rdf:type owl:Restriction ;
                                                                                                                owl:onProperty obo:BFO_0000054 ; # has realization
                                                                                                                owl:someValuesFrom prov:Activity
                                                                                                              ]
                                                                                                            ) ;
                                                                                         rdf:type owl:Class
                                                                                       ]
                                                                  ]
                                                                ) ;
                                             rdf:type owl:Class
                                           ]
                                         )
                           ] ;
               rdfs:comment  "An agent, if it's a material entity, has a role, that, if realized, is realized in an activity taking place"@en .


prov:Activity  rdfs:subClassOf   [ rdf:type owl:Restriction ;
                                    owl:onProperty obo:RO_0000057 ;  # has participant
                                    owl:someValuesFrom prov:Agent .
                                 ] .