@prefix rdf:    <http://www.w3.org/1999/02/22-rdf-syntax-ns#> .
@prefix rdfs:   <http://www.w3.org/2000/01/rdf-schema#> .
@prefix owl:    <http://www.w3.org/2002/07/owl#> .
@prefix prov:   <http://www.w3.org/ns/prov#> .
@prefix obo:    <http://purl.obolibrary.org/obo/> .
@prefix dc:     <http://purl.org/dc/elements/1.1/> .
@prefix sssom:  <https://w3id.org/sssom/> .
@base <https://raw.githubusercontent.com/BFO-Mappings/BFO-Mappings/main/PROV/prov-ro-directmappings.ttl> .

<https://raw.githubusercontent.com/BFO-Mappings/BFO-Mappings/main/PROV/prov-ro-directmappings.ttl>
  a                    owl:Ontology;
  rdfs:label           "Relation Ontology (RO) mappings for W3C PROVenance Interchange Ontology (PROV-O)"@en ;
  owl:versionInfo      "2023-10-08"@en ;
  owl:versionIRI       <http://www.w3.org/ns/prov-ro-directmappings-20230718> ;
  owl:imports          <https://raw.githubusercontent.com/BFO-Mappings/BFO-Mappings/main/PROV/prov-bfo-directmappings.ttl> ;
  rdfs:comment          "This mapping depends on the imported PROV-O to BFO mapping." ;
  dc:contributor        "Sydney Cohen" , "Giacomo De Colle" , "Austin Liebers" , "Tim Prudhomme" , "Alec Sculley" , "Peihong Karl Xie" ;
  rdfs:seeAlso         <http://www.w3.org/ns/prov> ,
                        <https://github.com/BFO-Mappings/BFO-Mappings> ,
                        <https://obofoundry.org/ontology/ro.html> ;
.

# Class mappings and property restrictions
prov:Agent rdf:type owl:Class .
[]  rdf:type owl:Axiom ;
    owl:annotatedSource   prov:Agent ;
    owl:annotatedProperty rdfs:subClassOf ; 
    owl:annotatedTarget   [ owl:intersectionOf ( obo:BFO_0000040 # material entity
                                                  [ rdf:type owl:Restriction ;
                                                    owl:onProperty obo:BFO_0000056 ; # participates in at some time
                                                    owl:someValuesFrom prov:Activity
                                                  ]
                                                  [ rdf:type owl:Restriction ;
                                                    owl:onProperty obo:RO_0000087 ;
                                                    owl:someValuesFrom [ owl:intersectionOf ( obo:BFO_0000023 # role
                                                                                              [ rdf:type owl:Restriction ;
                                                                                                owl:onProperty obo:BFO_0000054 ; # realized in / has realization
                                                                                                owl:someValuesFrom prov:Activity
                                                                                              ]
                                                                                            ) ;
                                                                        rdf:type owl:Class
                                                                      ]
                                                  ]
                                                ) ;
                            rdf:type owl:Class
                          ] ;
    sssom:object_label    "material entity that participates in some Activity at some time and has a role realized in that Activity" ;
    rdfs:comment "TODO"@en .


# Object Property mappings
prov:influenced rdf:type owl:ObjectProperty .
[]  rdf:type owl:Axiom ;
    owl:annotatedSource   prov:influenced ;
    owl:annotatedProperty rdfs:subPropertyOf ;
    owl:annotatedTarget   obo:RO_0002410 ;
    sssom:object_label    "casually related to" ;
    rdfs:comment "An entity may influence another entity and this is a causal relation."@en .


prov:wasAttributedTo rdf:type owl:ObjectProperty .
[]  rdf:type owl:Axiom ;
    owl:annotatedSource   prov:wasAttributedTo ;
    owl:annotatedProperty rdfs:subPropertyOf ;
    owl:annotatedTarget   obo:RO_0002559 ;
    sssom:object_label    "causally influenced by" ;
    rdfs:comment "An entity may be attributed to an agent, and this is a causal influence by the agent"@en .


prov:alternateOf rdf:type owl:ObjectProperty .
[]  rdf:type owl:Axiom ;
    owl:annotatedSource   prov:alternateOf ;
    owl:annotatedProperty rdfs:subPropertyOf ;
    owl:annotatedTarget   obo:RO_0002559 ;
    sssom:object_label    "causally influenced by" ;
    rdfs:comment "An entity may be an alternate of an entity, and this is a causal relation."@en .


prov:wasDerivedFrom rdf:type owl:ObjectProperty .
[]  rdf:type owl:Axiom ;
    owl:annotatedSource   prov:wasDerivedFrom ;
    owl:annotatedProperty rdfs:subPropertyOf ;
    owl:annotatedTarget   obo:RO_0002559 ;
    sssom:object_label    "causally influenced by" ;
    rdfs:comment "An entity may be derived from an entity, being causally influenced by it."@en .


prov:wasEndedBy rdf:type owl:ObjectProperty .
[]  rdf:type owl:Axiom ;
    owl:annotatedSource   prov:wasEndedBy ;
    owl:annotatedProperty rdfs:subPropertyOf ;
    owl:annotatedTarget   obo:RO_0000057 ;
    sssom:object_label    "has participant" ;
    rdfs:comment "A process has a (non spatial region) continuant as a participant. An activity is a process that may be ended by a prov:Entity as a participant."@en ;
    rdfs:comment "This mapping overlaps the same mapping to BFO's 'has participant at some time' but is included for increased interoperability." .


prov:wasStartedBy rdf:type owl:ObjectProperty .
[]  rdf:type owl:Axiom ;
    owl:annotatedSource   prov:wasStartedBy ;
    owl:annotatedProperty rdfs:subPropertyOf ;
    owl:annotatedTarget   obo:RO_0000057 ;
    sssom:object_label    "has participant" ;
    rdfs:comment "A process has a (non spatial region) continuant as a participant. An activity is a process that may be started by a prov:Entity as a participant."@en ;
    rdfs:comment "This mapping overlaps the same mapping to BFO's 'has participant at some time' but is included for increased interoperability." .


prov:wasAssociatedWith rdf:type owl:ObjectProperty .
[]  rdf:type owl:Axiom ;
    owl:annotatedSource   prov:wasAssociatedWith ;
    owl:annotatedProperty rdfs:subPropertyOf ;
    owl:annotatedTarget   obo:RO_0000057 ;
    sssom:object_label    "has participant" ;
    rdfs:comment "A process has a (non spatial region) continuant as a participant. An activity is a process that may be associated with a prov:Entity as a participant."@en ;
    rdfs:comment "This mapping overlaps the same mapping to BFO's 'has participant at some time' but is included for increased interoperability." .


prov:invalidated rdf:type owl:ObjectProperty .
[]  rdf:type owl:Axiom ;
    owl:annotatedSource   prov:invalidated ;
    owl:annotatedProperty rdfs:subPropertyOf ;
    owl:annotatedTarget   obo:RO_0000057 ;
    sssom:object_label    "has participant" ;
    rdfs:comment "A process has a (non spatial region) continuant as a participant. An activity is a process that may be invalidated by a prov:Entity as a participant."@en ;
    rdfs:comment "This mapping overlaps the same mapping to BFO's 'has participant at some time' but is included for increased interoperability." .


prov:used rdf:type owl:ObjectProperty .
[]  rdf:type owl:Axiom ;
    owl:annotatedSource   prov:used ;
    owl:annotatedProperty rdfs:subPropertyOf ;
    owl:annotatedTarget   obo:RO_0000057 ;
    sssom:object_label    "has participant" ;
    rdfs:comment "A process has a (non spatial region) continuant as a participant. An activity is a process that may use a prov:Entity as a participant."@en ;
    rdfs:comment "This mapping overlaps the same mapping to BFO's 'has participant at some time' but is included for increased interoperability." .


prov:generated rdf:type owl:ObjectProperty .
[]  rdf:type owl:Axiom ;
    owl:annotatedSource   prov:generated ;
    owl:annotatedProperty rdfs:subPropertyOf ;
    owl:annotatedTarget   obo:RO_0000057 ;
    sssom:object_label    "has participant" ;
    rdfs:comment "An activity is a process that may be generated by a prov:Entity as a participant."@en ;
    rdfs:comment "This mapping overlaps the same mapping to BFO's 'has participant at some time' but is included for increased interoperability." .


prov:wasInvalidatedBy rdf:type owl:ObjectProperty .
[]  rdf:type owl:Axiom ;
    owl:annotatedSource   prov:wasInvalidatedBy ;
    owl:annotatedProperty rdfs:subPropertyOf ;
    owl:annotatedTarget   obo:RO_0000056 ;
    sssom:object_label    "participates in" ;
    rdfs:comment "An entity (non-spatial region continuant) may participate in its invalidation by an activity (process)"@en ;
    rdfs:comment "This mapping overlaps the same mapping to BFO's 'participates in at some time' but is included for increased interoperability." .


prov:wasGeneratedBy rdf:type owl:ObjectProperty .
[]  rdf:type owl:Axiom ;
    owl:annotatedSource   prov:wasGeneratedBy ;
    owl:annotatedProperty rdfs:subPropertyOf ;
    owl:annotatedTarget   obo:RO_0000056 ;
    sssom:object_label    "participates in" ;
    rdfs:comment "An entity (non-spatial region continuant) may participate in its generation by an activity (process)"@en ;
    rdfs:comment "This mapping overlaps the same mapping to BFO's 'participates in at some time' but is included for increased interoperability." .


prov:wasInformedBy rdf:type owl:ObjectProperty .
[]  rdf:type owl:Axiom ;
    owl:annotatedSource   prov:wasInformedBy ;
    owl:annotatedProperty rdfs:subPropertyOf ;
    owl:annotatedTarget   obo:RO_0002501 ;
    sssom:object_label    "causal relation between processes" ;
    rdfs:comment "An activity may inform an activity. Both are processes and this is a causal relation."@en .


prov:hadGeneration rdf:type owl:ObjectProperty .
[]  rdf:type owl:Axiom ;
    owl:annotatedSource   prov:hadGeneration ;
    owl:annotatedProperty rdfs:subPropertyOf ;
    owl:annotatedTarget   obo:RO_0002501 ;
    sssom:object_label    "causal relation between processes" ;
    rdfs:comment "An activity may generate another activity. Both are processes and this is a causal relation."@en .


prov:hadUsage rdf:type owl:ObjectProperty .
[]  rdf:type owl:Axiom ;
    owl:annotatedSource   prov:hadUsage ;
    owl:annotatedProperty rdfs:subPropertyOf ;
    owl:annotatedTarget   obo:RO_0002501 ;
    sssom:object_label    "causal relation between processes" ;
    rdfs:comment "A derivation may use a usage. Both are processes and this is a causal relation."@en .

prov:hadActivity rdf:type owl:ObjectProperty .
[]  rdf:type owl:Axiom ;
    owl:annotatedSource   prov:hadActivity ;
    owl:annotatedProperty rdfs:subPropertyOf ;
    owl:annotatedTarget   obo:RO_0002501 ;
    sssom:object_label    "causal relation between processes" ;
    rdfs:comment "An influence that's related to an activity in this context is causally related to it, where both are processes."@en .

prov:qualifiedAssociation rdf:type owl:ObjectProperty .
[]  rdf:type owl:Axiom ;
    owl:annotatedSource   prov:qualifiedAssociation ;
    owl:annotatedProperty rdfs:subPropertyOf ;
    owl:annotatedTarget   obo:RO_0002501 ;
    sssom:object_label    "causal relation between processes" ;
    rdfs:comment "An activity may be associated with an activity. Both are processes and this is a causal relation."@en .


prov:qualifiedCommunication rdf:type owl:ObjectProperty .
[]  rdf:type owl:Axiom ;
    owl:annotatedSource   prov:qualifiedCommunication ;
    owl:annotatedProperty rdfs:subPropertyOf ;
    owl:annotatedTarget   obo:RO_0002501 ;
    sssom:object_label    "causal relation between processes" ;
    rdfs:comment "An activity may communicate another activity. Both are processes and this is a causal relation. For example: A wasInfomedBy B = A and B are both prov:activities, and A was causally related to B such that A utilizes a provenance_entity that wasGeneratedBy B"@en .


prov:qualifiedStart rdf:type owl:ObjectProperty .
[]  rdf:type owl:Axiom ;
    owl:annotatedSource   prov:qualifiedStart ;
    owl:annotatedProperty rdfs:subPropertyOf ;
    owl:annotatedTarget   obo:RO_0002501 ;
    sssom:object_label    "causal relation between processes" ;
    rdfs:comment "An activity may start an activity. Both are processes and this is a causal relation."@en .


prov:hadMember rdf:type owl:ObjectProperty .
[]  rdf:type owl:Axiom ;
    owl:annotatedSource   prov:hadMember ;
    owl:annotatedProperty rdfs:subPropertyOf ;
    owl:annotatedTarget   obo:RO_0002351 ;
    sssom:object_label    "had member" ;
    rdfs:comment "TODO: Establish a relationship between similar BFO/RO and PROV terms - PROV term is more specific than the RO has member relation, and hence is a subclass of the RO term "@en .
